Translation.v
@@ -1,57 +1,48 @@
 Add LoadPath "vst".
 Require Import CpdtTactics.
 Require Import Types.
-Require Import ProgramLogic.
 Require Import Language.
+Require Export ProgramLogic.
 Require Import Subst.
 Require Import List.
 Import ListNotations.
-Require Import msl.msl_direct.
 Require Import Coq.Unicode.Utf8.
 
 Set Implicit Arguments.
 
-Open Scope pred.
+Open Scope logic.
 
-Definition sep_base (x:expr) (t:base_type) : pred world :=
-  EX v : (base_of_type t), (fun s => (eval s x = (val_of_base t v))).
+Definition sep_base (x:expr) (t:base_type) : assert :=
+  EX v : (base_of_type t), (fun s => !!(eval s x = (val_of_base t v))) && emp.
 
-Fixpoint sep_pred (p:reft_prop) : pred world :=
+Fixpoint sep_pred (p:reft_prop) : assert :=
   match p with
     | tt_r  => TT
     | rel_r e1 o e2 =>
       match o with
-        | eq_brel => (fun s => eval s e1 = eval s e2)
+        | eq_brel => (fun s => !!(eval s e1 = eval s e2))
       end
     | not_r p => (sep_pred p) --> FF
     | and_r p1 p2 => sep_pred p1 && sep_pred p2
     | or_r p1 p2 => sep_pred p1 || sep_pred p2
-  end.
+  end && emp.
 
-Definition sep_ty (x:expr) (t:reft_type) : pred world :=
+Definition sep_ty (x:expr) (t:reft_type) : assert :=
   match t with
   | mkReft_type b p => sep_base x b && (sep_pred (subst (subst_one ν x) p))
-  end.
+  end && emp.
 
-(* Definition sep_base_e (e:expr) (t:base_type) : pred world := *)
-(*   EX v : (base_of_type t), (fun s => (eval s e = (val_of_base t v))). *)
-
-(* Definition sep_ty_e (e:expr) (t:reft_type) : pred world := *)
-(*   match t with *)
-(*   | mkReft_type b p => sep_base_e e b && (sep_pred (subst (subst_one ν e) p)) *)
-(*   end. *)
-
-Fixpoint sep_env (Γ : type_env) : pred world :=
+Fixpoint sep_env (Γ : type_env) : assert :=
   match Γ with
     | nil => TT
     | (x,t) :: Γ' => sep_ty (var_e x) t && sep_env Γ'
-  end.
+  end && emp.
 
-Fixpoint sep_guards (Δ : guards) : pred world :=
+Fixpoint sep_guards (Δ : guards) : assert :=
   match Δ with
     | nil => TT
     | p :: Δ' => sep_pred p && sep_guards Δ'
-  end.
+  end && emp.
 
 Definition sep_schema (f:pname) (s:stmt) (S:proc_schema) : procspec := 
   match S with
@@ -67,3 +58,60 @@ Fixpoint sep_proc_env (Φ : proc_env) : procspecs :=
 
 Definition disj_subst Γ (θ : var -> expr) :=
   θ ν = (var_e ν) /\ forall x, var_in x Γ -> θ x = (var_e x).
+
+Lemma sep_base_pure : 
+  forall x t, 
+    pure (sep_base x t).
+Proof.
+  intros.
+  unfold pure.
+  unfold sep_base.
+  rewrite <- exp_andp1.
+  apply andp_left2.
+  apply derives_refl.
+Qed.
+
+Lemma sep_pred_pure :
+  forall p,
+    pure (sep_pred p).
+Proof.
+  intros.
+  unfold pure.
+  destruct p;
+  unfold sep_pred; fold sep_pred; apply andp_left2; apply derives_refl.
+Qed.
+
+Lemma sep_ty_pure :
+  forall x t,
+    pure (sep_ty x t).
+Proof.
+  intros.
+  unfold pure, sep_ty.
+  destruct t.
+  repeat apply andp_left1.
+  apply sep_base_pure.
+Qed.
+
+Lemma sep_env_pure :
+  forall g,
+    pure (sep_env g).
+Proof.
+  intros.
+  unfold pure.
+  destruct g.
+  apply andp_left2. apply derives_refl.
+  unfold sep_env. fold sep_env.
+  apply andp_left2. apply derives_refl.
+Qed.
+
+Lemma sep_guard_pure :
+  forall g,
+    pure (sep_guards g).
+Proof.
+  intros.
+  unfold pure, sep_guards.
+  destruct g.
+  normalize.
+  apply andp_left2.
+  apply derives_refl.
+Qed.
