EvalLemmas.v
@@ -1,5 +1,7 @@
 Add LoadPath "vst".
-Require Import msl.msl_direct.
+Require Import msl.Coqlib2.
+Require Import msl.log_normalize.
+Require Import msl.eq_dec.
 Require Import Coq.Unicode.Utf8.
 Require Import Coq.Program.Equality.
 
@@ -15,63 +17,88 @@ Require Import Tactics.
 Open Scope pred.
 
 Lemma var_val :
-  forall Γ x b φ w,  (x,{ ν : b | φ}) ∈ Γ ->
-                       sep_env Γ w ->
-                       (EX v : (base_of_type b),
-                               (fun s => eval s (var_e x) = val_of_base b v)) w.
+  forall Γ x b φ, 
+    (x,{ ν : b | φ}) ∈ Γ ->
+    sep_env Γ |-- (EX v : (base_of_type b),
+                          (fun s => !!(eval s (var_e x) = val_of_base b v))).
 Proof.
   induction Γ. 
-  crush_sep False fail.
-  crush_sep False fail.
-  fold (subst_pred (subst_one ν (var_e x)) (sep_base (var_e ν) b0) w) in H.
-  unfold subst_one in H.
-  unfold subst_pred in H.
-  unfold sep_base in H.
+  intuition.
+  intuition.
   destruct H.
-  destruct b0.
-  simpl in *.
-  exists x0.
-  foo.
-  specialize (IHΓ x b0 φ w).
-  destruct b0. simpl in *.
-  apply IHΓ; assumption.
+  + apply andp_left1. 
+    apply andp_left1.
+    apply andp_left1.
+    destruct b.
+    inversion H. subst. 
+    apply andp_left1.
+    apply exp_left.
+    intro bb.
+    apply andp_left1.
+    apply (exp_right bb).
+    apply derives_refl.
+  + apply andp_left1.
+    apply andp_left2.
+    fold sep_env.
+    apply IHΓ with (φ := φ).
+    assumption.
 Qed.
 
 Lemma var_eval :
-  forall Γ x b φ w, (x, { ν : b | φ }) ∈ Γ -> sep_env Γ w -> 
-                    (EX v : value, (fun s => eval s (var_e x) = v)) w.
+  forall Γ x b φ, 
+    (x, { ν : b | φ }) ∈ Γ -> 
+    sep_env Γ |-- (EX v : value, (fun s => !!(eval s (var_e x) = v))).
 Proof.
-  crush_sep False fail.
-  apply var_val with (x := x) (b := b) (φ := φ)in H0 .
-  destruct H0.
-  destruct b. simpl in *. exists (int_v x0). assumption.
+  intros.
+  pose (var_val Γ x b φ H).
+  apply derives_trans with (Q := EX x0 : base_of_type b, (fun s => !!(eval s (var_e x) = val_of_base b x0))).
   assumption.
+  destruct b.
+  apply exp_left.
+  intro xv.
+  simpl.
+  intro w.
+  apply prop_left.
+  intro.
+  rewrite H0.
+  simpl in xv.
+  apply (exp_right (int_v xv)).
+  apply prop_right.
+  reflexivity.
 Qed.
 
 Lemma expr_eval :
-  forall Γ Ξ e b φ w,
-    sep_env Γ w -> expr_type Γ Ξ e { ν : b | φ } ->
-                (EX v : value, (fun s => eval s e = v)) w.
+  forall Γ Ξ e b φ,
+    expr_type Γ Ξ e { ν : b | φ } ->
+    sep_env Γ |-- (EX v : value, (fun s => !!(eval s e = v))).
 Proof.
-  autounfold in *. intros.
-  induction H0.
-  * simpl. exists v. reflexivity.
+  intros.
+  induction H.
+  * apply (exp_right v). simpl. intro. apply prop_right. reflexivity.
   * apply var_eval with (Γ := Γ) (b := τ) (φ := φ0); assumption.
-  * apply IHexpr_type; assumption.
+  * apply IHexpr_type. 
 Qed.
 
 Lemma expr_eval_ty :
-  forall Γ Ξ e b φ w,
-    sep_env Γ w -> expr_type Γ Ξ e { ν : b | φ } ->
-      (EX v : base_of_type b , (fun s => eval s e = val_of_base b v)) w.
+  forall Γ Ξ e b φ,
+    expr_type Γ Ξ e { ν : b | φ } ->
+    sep_env Γ |-- 
+      (EX v : base_of_type b , (fun s => !!(eval s e = val_of_base b v))).
 Proof.
-  autounfold in *. intros.
+  intros.
   apply expr_eval with (e := e) (b := b) (φ := φ) (Ξ := Ξ) in H.
-  destruct H.
+  apply derives_trans with 
+    (Q := EX v : value, (fun s => !!(eval s e = v))).
+  assumption.
+  apply exp_left. intro vv.
   destruct b.
-  destruct x.
-  exists n. 
-  apply H.
+  destruct vv.
+  simpl.
+  intro w.
+  apply prop_left.
+  intro.
+  apply (exp_right n).
+  apply prop_right.
   assumption.
 Qed.
 
@@ -85,63 +112,69 @@ Proof.
 Qed.
 
 Lemma subst_env_eq_expr :
-  forall G Grds b x e w φ, 
+  forall G Grds b x e φ, 
     expr_type G Grds e { ν : b | φ } ->
-    sep_env G w ->
-    (subst_pred (subst_one x e) (sep_env G)) w ->
-    subst_pred (subst_one x e) (sep_env ((x, { ν : b | var_e ν .= e }) :: G)) w.
+    sep_env G && 
+    (subst_pred (subst_one x e) (sep_env G))
+    |-- subst_pred (subst_one x e) (sep_env ((x, { ν : b | var_e ν .= e }) :: G)).
 Proof.
-  intros G Grds b x e w φ etype senv H.
-  pose (expr_eval_ty G Grds e b φ w senv etype) as H0.
+  intros.
+  pose (expr_eval_ty G Grds e b φ H).
   rewrite subst_env_cons.
-  split. {
-    split. {
-      unfold subst_pred.
-      unfold subst_one.
-      unfold sep_ty.
-      unfold sep_base.
-      unfold subst_one. 
-      destruct H0.
-      exists x0.
-      simpl.
-      destruct (eq_dec ν ν).
-      + simpl.
-        destruct (eq_dec x x). 
-        * assumption. 
-        * contradiction n; reflexivity. 
-      + contradiction n; reflexivity.
-    } 
-    {
-      unfold sep_pred.
-      unfold subst_one.
-      simpl in *.
-      unfold Subst.subst, Subst_var_expr.
-      simpl.
-      destruct (eq_dec ν ν).
-      simpl.
-      destruct e.
-      destruct (eq_dec x x).
-      simpl.
-      reflexivity.
-      contradiction n. reflexivity.
-      destruct (eq_dec x x). simpl.
-      destruct (eq_dec v ν). simpl.
-      destruct (eq_dec x x). reflexivity.
-      contradiction n.
-      simpl. 
-      destruct (eq_dec v x). 
-      reflexivity. 
-      reflexivity. 
-      contradiction n. 
-      reflexivity.
-      exfalso. 
-        apply exfalso_etype_fun with (G := G) (Ξ := Grds) (f := p) (e1 := e1) (e2 := e2) (T := { ν : b | φ }).
-      assumption.
-      contradiction n.
-      reflexivity.
-    } 
-  }
-  {
+  apply derives_trans with (Q := sep_env G && subst_pred (subst_one x e) (sep_env G) && emp).
+  apply andp_right. normalize. apply andp_left1. apply sep_env_pure.
+  apply andp_derives.
+  apply andp_derives.
+  unfold sep_ty.
+  destruct {ν : b | var_e ν .= e} eqn: T.
+  inversion T. subst.
+  rewrite subst_distr_andp.
+  apply andp_right.
+  apply derives_trans with 
+   (Q := (EX v : base_of_type reft_base, (fun s => !!(eval s e = val_of_base reft_base v))) && emp).
+    apply andp_right.
     assumption.
-  }
+    apply sep_env_pure.
+    unfold sep_env. 
+    rewrite exp_andp1.
+    apply exp_left. intro v. intro w. 
+    (* apply prop_left. intro F. *)
+    unfold sep_base, subst_one, subst, Subst_pred, subst_pred.
+    simpl.
+    apply andp_right.
+    apply (exp_right v). 
+    destruct (eq_dec x x). 
+      apply derives_refl.
+      congruence.
+    apply andp_derives.
+    unfold subst, Subst_pred, subst_pred. simpl.
+    unfold subst, Subst_pred, Subst_var_expr, subst_pred.
+    destruct (eq_dec ν ν).
+    simpl.
+    destruct e.
+    simpl.
+    destruct (eq_dec x x).
+    simpl.
+    normalize.
+    normalize.
+    congruence.
+    normalize.
+    destruct (eq_dec x x).
+    simpl.
+    destruct (eq_dec v0 ν).
+    simpl.
+    destruct (eq_dec x x).
+    reflexivity.
+    congruence.
+    simpl.
+    destruct (eq_dec v0 x).
+    reflexivity.
+    reflexivity.
+    congruence.
+    exfalso; eapply exfalso_etype_fun; eauto.
+    congruence.
+    normalize.
+    apply sep_env_pure.
+    normalize.
+    normalize.
 Qed.
